cava/Cava/Util/If.v
@@ -1,0 +1,24 @@
+(****************************************************************************)
+(* Copyright 2021 The Project Oak Authors                                   *)
+(*                                                                          *)
+(* Licensed under the Apache License, Version 2.0 (the "License")           *)
+(* you may not use this file except in compliance with the License.         *)
+(* You may obtain a copy of the License at                                  *)
+(*                                                                          *)
+(*     http://www.apache.org/licenses/LICENSE-2.0                           *)
+(*                                                                          *)
+(* Unless required by applicable law or agreed to in writing, software      *)
+(* distributed under the License is distributed on an "AS IS" BASIS,        *)
+(* WITHOUT WARRANTIES OR CONDITIONS OF ANY KIND, either express or implied. *)
+(* See the License for the specific language governing permissions and      *)
+(* limitations under the License.                                           *)
+(****************************************************************************)
+
+Lemma apply_if {A B} (f : A -> B) (b : bool) x y : f (if b then x else y) = if b then f x else f y.
+Proof. destruct b; reflexivity. Qed.
+
+Lemma fst_if {A B} (b : bool) (x y : A * B) : fst (if b then x else y) = if b then fst x else fst y.
+Proof. apply apply_if. Qed.
+Lemma snd_if {A B} (b : bool) (x y : A * B) : snd (if b then x else y) = if b then snd x else snd y.
+Proof. apply apply_if. Qed.
+Hint Rewrite @fst_if @snd_if using solve [eauto] : tuple_if.
