investigations/cava2/ExprProperties.v
@@ -1,0 +1,78 @@
+(****************************************************************************)
+(* Copyright 2021 The Project Oak Authors                                   *)
+(*                                                                          *)
+(* Licensed under the Apache License, Version 2.0 (the "License")           *)
+(* you may not use this file except in compliance with the License.         *)
+(* You may obtain a copy of the License at                                  *)
+(*                                                                          *)
+(*     http://www.apache.org/licenses/LICENSE-2.0                           *)
+(*                                                                          *)
+(* Unless required by applicable law or agreed to in writing, software      *)
+(* distributed under the License is distributed on an "AS IS" BASIS,        *)
+(* WITHOUT WARRANTIES OR CONDITIONS OF ANY KIND, either express or implied. *)
+(* See the License for the specific language governing permissions and      *)
+(* limitations under the License.                                           *)
+(****************************************************************************)
+
+Require Import Coq.Lists.List.
+Require Import Coq.NArith.NArith.
+Require Import coqutil.Tactics.Tactics.
+Require Import Cava.Util.List.
+Require Import Cava.Util.Tactics.
+Require Import Cava.Expr.
+Require Import Cava.Primitives.
+Require Import Cava.Semantics.
+Require Import Cava.Types.
+
+Lemma step_vec_as_tuple_cons {t n} (xs : list (denote_type t)) :
+  step (vec_as_tuple (t:=t) (n:=S n)) tt (xs, tt)
+  = (tt, (hd default xs, snd (step (vec_as_tuple (t:=t) (n:=n)) tt (tl xs, tt)))).
+Proof. reflexivity. Qed.
+Hint Rewrite @step_vec_as_tuple_cons using solve [eauto] : stepsimpl.
+
+Lemma step_vec_as_tuple_one {t} (xs : list (denote_type t)):
+  step (vec_as_tuple (t:=t) (n:=0)) tt (xs, tt) = (tt, hd default xs).
+Proof. reflexivity. Qed.
+Hint Rewrite @step_vec_as_tuple_one using solve [eauto] : stepsimpl.
+
+Ltac stepsimpl :=
+  repeat first [ progress
+                   cbn [fst snd step denote_type absorb_any
+                            split_absorbed_denotation combine_absorbed_denotation
+                            unary_semantics binary_semantics eqb ]
+               | progress autorewrite with stepsimpl ].
+
+Lemma step_index {t n i} (x : denote_type (Vec t n))
+      (idx : denote_type (BitVec i)) :
+  step (@index _ t n i) tt (x, (idx, tt))
+  = (tt, nth (N.to_nat idx) (List.resize default n x) default).
+Proof. reflexivity. Qed.
+Hint Rewrite @step_index using solve [eauto] : stepsimpl.
+
+Lemma step_uncons {t n}  (x : denote_type [Vec t (S n)]) :
+  step (@uncons _ t n) tt x = (tt, (hd default (fst x), tl (fst x))).
+Proof. destruct x; reflexivity. Qed.
+Hint Rewrite @step_uncons using solve [eauto] : stepsimpl.
+
+Lemma step_stateless {i o} (f : Circuit [] i o) (x : denote_type i) :
+  step f tt x = (tt, snd (step f tt x)).
+Proof.
+  rewrite (surjective_pairing (step f tt x)).
+  destruct (fst (step f tt x)). reflexivity.
+Qed.
+
+Lemma step_map2 {t u v n} (f : Circuit [] [t;u] v)
+      (x : denote_type [Vec t n; Vec u n]) :
+  step (@Expr.map2 _ t u v n f) tt x
+  = (tt, List.map2 (fun (x1 : denote_type t) (x2 : denote_type u) =>
+                      snd (step f tt (x1,(x2,tt))))
+                   (List.resize default n (fst x))
+                   (List.resize default n (fst (snd x)))).
+Proof.
+  revert x f; induction n; cbn [Expr.map2]; stepsimpl;
+    intros; destruct_products; logical_simplify; stepsimpl;
+      [ rewrite resize_0; reflexivity | ].
+  rewrite step_stateless, IHn.
+  rewrite !resize_succ. reflexivity.
+Qed.
+Hint Rewrite @step_map2 using solve [eauto] : stepsimpl.
